Implemented semantics for IntegerTestNode. Changed the definition for conditional expression evaluation to make some proofs easier

Graph/IRNodes.thy
@@ -69,6 +69,7 @@ datatype (discs_sels) IRNode =
   | IntegerBelowNode (ir_x: "INPUT") (ir_y: "INPUT") 
   | IntegerEqualsNode (ir_x: "INPUT") (ir_y: "INPUT") 
   | IntegerLessThanNode (ir_x: "INPUT") (ir_y: "INPUT") 
+  | IntegerTestNode (ir_x: "INPUT") (ir_y: "INPUT")
   | InvokeNode (ir_nid: ID) (ir_callTarget: "INPUT_EXT") (ir_classInit_opt: "INPUT option") (ir_stateDuring_opt: "INPUT_STATE option") (ir_stateAfter_opt: "INPUT_STATE option") (ir_next: "SUCC") 
   | InvokeWithExceptionNode (ir_nid: ID) (ir_callTarget: "INPUT_EXT") (ir_classInit_opt: "INPUT option") (ir_stateDuring_opt: "INPUT_STATE option") (ir_stateAfter_opt: "INPUT_STATE option") (ir_next: "SUCC") (ir_exceptionEdge: "SUCC") 
   | IsNullNode (ir_value: "INPUT") 
@@ -160,6 +161,8 @@ fun inputs_of :: "IRNode \<Rightarrow> ID list" where
   "inputs_of (IntegerEqualsNode x y) = [x, y]" |
   inputs_of_IntegerLessThanNode:
   "inputs_of (IntegerLessThanNode x y) = [x, y]" |
+  inputs_of_IntegerTestNode:
+  "inputs_of (IntegerTestNode x y) = [x, y]" |
   inputs_of_InvokeNode:
   "inputs_of (InvokeNode nid0 callTarget classInit stateDuring stateAfter next) = callTarget # (opt_to_list classInit) @ (opt_to_list stateDuring) @ (opt_to_list stateAfter)" |
   inputs_of_InvokeWithExceptionNode:
@@ -271,6 +274,8 @@ fun successors_of :: "IRNode \<Rightarrow> ID list" where
   "successors_of (IntegerEqualsNode x y) = []" |
   successors_of_IntegerLessThanNode:
   "successors_of (IntegerLessThanNode x y) = []" |
+  successors_of_IntegerTestNode:
+  "successors_of (IntegerTestNode x y) = []" |
   successors_of_InvokeNode:
   "successors_of (InvokeNode nid0 callTarget classInit stateDuring stateAfter next) = [next]" |
   successors_of_InvokeWithExceptionNode:
