Semantics/IRStepThms.thy
@@ -91,21 +91,21 @@ proof (induction rule: "step.induct")
   have notif: "\<not>(is_IfNode (kind g nid))"
     by (metis is_IfNode_def SequentialNode.hyps(1) is_sequential_node.simps(19))
   have notend: "\<not>(is_AbstractEndNode (kind g nid))"
-    by (metis is_AbstractEndNode.simps SequentialNode.hyps(1) is_sequential_node.simps(15,29)
+    by (metis is_AbstractEndNode.simps SequentialNode.hyps(1) is_sequential_node.simps(15,30)
         is_EndNode.elims(2) is_LoopEndNode_def)
   have notnew: "\<not>(is_NewInstanceNode (kind g nid))"
-    by (metis is_NewInstanceNode_def SequentialNode.hyps(1) is_sequential_node.simps(35))
+    by (metis is_NewInstanceNode_def SequentialNode.hyps(1) is_sequential_node.simps(36))
   have notload: "\<not>(is_LoadFieldNode (kind g nid))"
-    by (metis is_LoadFieldNode_def SequentialNode.hyps(1) is_sequential_node.simps(27))
+    by (metis is_LoadFieldNode_def SequentialNode.hyps(1) is_sequential_node.simps(28))
   have notstore: "\<not>(is_StoreFieldNode (kind g nid))"
-    by (metis is_StoreFieldNode_def SequentialNode.hyps(1) is_sequential_node.simps(46))
+    by (metis is_StoreFieldNode_def SequentialNode.hyps(1) is_sequential_node.simps(47))
   have notdivrem:  "\<not>(is_IntegerDivRemNode (kind g nid))"
-    by (metis is_IntegerDivRemNode.simps SequentialNode.hyps(1) is_sequential_node.simps(44,45) 
+    by (metis is_IntegerDivRemNode.simps SequentialNode.hyps(1) is_sequential_node.simps(45,46)
         is_SignedDivNode_def is_SignedRemNode_def)
   from notif notend notnew notload notstore notdivrem
   show ?case 
-    by (smt (verit) SequentialNode step.cases IRNode.disc(1102,2367) IRNode.discI(32) Pair_inject
-        is_sequential_node.simps(17,19,44,45))
+    by (smt (verit) SequentialNode step.cases is_sequential_node.simps(17,19,28,36,45,46,47)
+        Pair_inject IRNode.discI(32))
 next
   case (FixedGuardNode nid cond before "next" condE m p val h)
   have notseq: "\<not>(is_sequential_node (kind g nid))"
@@ -113,9 +113,9 @@ next
   have notend: "\<not>(is_AbstractEndNode (kind g nid))"
     by (simp add: FixedGuardNode.hyps(1))
   from notseq notend 
-  show ?case 
-    by (smt (verit) FixedGuardNode.hyps(1,5) IRNode.distinct(973,991,1013,1031,1033,1037) step.simps
-        IRNode.inject(10) Pair_inject)
+  show ?case
+    by (smt (verit) FixedGuardNode.hyps(1,5) IRNode.distinct(993,1013,1035,1053,1055,1059)
+        step.simps Pair_inject IRNode.inject(10))
 next
   case (IfNode nid cond tb fb m val "next" h)
   then have notseq: "\<not>(is_sequential_node (kind g nid))"
@@ -125,37 +125,36 @@ next
   have notdivrem: "\<not>(is_IntegerDivRemNode (kind g nid))" 
     by (simp add: IfNode.hyps(1))
   from notseq notend notdivrem show ?case
-    by (smt (verit) IRNode.inject(11,12) Pair_inject step.simps IfNode repDet evalDet step.simps
-        IRNode.distinct(973,1157,1179,1197,1199,1203))
+    by (smt (verit) IRNode.inject(11,12) Pair_inject step.simps IfNode repDet evalDet
+        IRNode.distinct(993,1183,1205,1223,1225,1229))
 next
   case (EndNodes nid merge i phis inputs m vs m' h)
   have notseq: "\<not>(is_sequential_node (kind g nid))"
-    by (metis is_EndNode.elims(2) is_LoopEndNode_def is_sequential_node.simps(15, 29) 
+    by (metis is_EndNode.elims(2) is_LoopEndNode_def is_sequential_node.simps(15,30)
         is_AbstractEndNode.simps EndNodes.hyps(1))
   have notif: "\<not>(is_IfNode (kind g nid))"
-    by (metis IRNode.distinct_disc(1164) is_AbstractEndNode.elims(2) EndNodes.hyps(1) is_IfNode_def
+    by (metis IRNode.distinct_disc(1189) is_AbstractEndNode.elims(2) EndNodes.hyps(1) is_IfNode_def
         is_EndNode.simps(13))
   have notref: "\<not>(is_RefNode (kind g nid))"
-    by (metis EndNodes.hyps(1) is_AbstractEndNode.simps is_EndNode.elims(2) is_LoopEndNode_def 
-        is_RefNode_def is_sequential_node.simps(7,15,29))
+    by (metis notseq is_RefNode_def is_sequential_node.simps(7))
   have notnew: "\<not>(is_NewInstanceNode (kind g nid))"
-    by (metis IRNode.distinct_disc(2008) is_EndNode.simps(33) is_NewInstanceNode_def 
+    by (metis IRNode.distinct_disc(2115) is_EndNode.simps(34) is_NewInstanceNode_def
         is_AbstractEndNode.simps EndNodes.hyps(1))
   have notload: "\<not>(is_LoadFieldNode (kind g nid))"
-    by (metis IRNode.distinct_disc(1812) is_EndNode.simps(22) is_LoadFieldNode_def EndNodes.hyps(1)
+    by (metis IRNode.distinct_disc(1920) is_EndNode.simps(23) is_LoadFieldNode_def EndNodes.hyps(1)
         is_AbstractEndNode.simps)
   have notstore: "\<not>(is_StoreFieldNode (kind g nid))"
-    by (metis IRNode.distinct_disc(2032) is_EndNode.simps(45) is_StoreFieldNode_def EndNodes.hyps(1)
+    by (metis IRNode.distinct_disc(2140) is_EndNode.simps(46) is_StoreFieldNode_def EndNodes.hyps(1)
         is_AbstractEndNode.simps)
   have notdivrem: "\<not>(is_IntegerDivRemNode (kind g nid))"
     using EndNodes.hyps(1) is_SignedDivNode_def is_SignedRemNode_def by auto
   have notfixedguard: "\<not>(is_FixedGuardNode (kind g nid))"
-    by (metis IRNode.distinct_disc(997) is_EndNode.simps(11) is_FixedGuardNode_def EndNodes.hyps(1)
+    by (metis IRNode.distinct_disc(1019) is_EndNode.simps(11) is_FixedGuardNode_def EndNodes.hyps(1)
         is_AbstractEndNode.simps)
   from notseq notif notref notnew notload notstore notdivrem notfixedguard
   show ?case 
-    by (smt (verit) repAllDet evalAllDet IRNode.disc(497) is_IfNode_def is_RefNode_def Pair_inject
-        is_LoadFieldNode_def is_NewInstanceNode_def is_StoreFieldNode_def step.cases EndNodes
+    by (smt (verit) IRNode.disc(497,506) repAllDet evalAllDet is_IfNode_def EndNodes step.cases
+        is_RefNode_def Pair_inject is_LoadFieldNode_def is_NewInstanceNode_def is_StoreFieldNode_def
         is_SignedDivNode_def is_SignedRemNode_def is_IntegerDivRemNode.elims(3))
 next
   case (NewInstanceNode nid f obj nxt h' ref h m' m)
@@ -175,8 +174,8 @@ next
     by (simp add: NewInstanceNode.hyps(1))
   from notseq notend notif notref notload notstore notdivrem
   show ?case 
-    by (smt (verit) NewInstanceNode step.cases IRNode.disc(1102, 2367) IRNode.discI(12) Pair_inject
-        IRNode.distinct(1013,2417,2419) IRNode.inject(32))
+    by (smt (verit) NewInstanceNode step.cases IRNode.disc(1102,1013,1178,2367,2417,2419,2466)
+        IRNode.discI(12) Pair_inject IRNode.distinct(1035,2525,2527) IRNode.inject(32,33))
 next
   case (LoadFieldNode nid f obj nxt m ref h v m')
   then have notseq: "\<not>(is_sequential_node (kind g nid))"
@@ -187,8 +186,9 @@ next
     by (simp add: LoadFieldNode.hyps(1))
   from notseq notend notdivrem
   show ?case 
-    by (smt (verit) LoadFieldNode step.cases repDet evalDet IRNode.inject(21) option.distinct(1)
-        IRNode.distinct(991,1157,1827,1845,1847,1851) Pair_inject Value.inject(2) option.inject)
+    by (smt (verit) LoadFieldNode step.cases repDet evalDet IRNode.inject(21,22) option.distinct(1)
+        IRNode.distinct(991,1013,1157,1183,1827,1845,1847,1851,1935,1953,1955,1959) Pair_inject
+        Value.inject(2) option.inject)
 next
   case (StaticLoadFieldNode nid f nxt h v m' m)
   then have notseq: "\<not>(is_sequential_node (kind g nid))"
@@ -199,8 +199,8 @@ next
     by (simp add: StaticLoadFieldNode.hyps(1))
   from notseq notend notdivrem
   show ?case  
-    by (smt (verit) StaticLoadFieldNode step.cases IRNode.inject(21) Pair_inject option.distinct(1)
-        IRNode.distinct(991,1157,1827,1845,1847,1851))
+    by (smt (verit) IRNode.distinct(991,1013,1157,1183,1827,1845,1847,1851,1935,1953,1955,1959)
+        IRNode.inject(21,22) StaticLoadFieldNode step.cases Pair_inject option.distinct(1))
 next
   case (StoreFieldNode nid f newval uu obj nxt m val ref h' h m')
   then have notseq: "\<not>(is_sequential_node (kind g nid))"
@@ -211,8 +211,9 @@ next
     by (simp add: StoreFieldNode.hyps(1))
   from notseq notend notdivrem
   show ?case 
-    by (smt (verit) StoreFieldNode step.cases repDet evalDet IRNode.inject(44) option.distinct(1)
-        IRNode.distinct(1037,1203,1851,2423,2711,2733) Value.inject(2) Pair_inject option.inject)
+    by (smt (verit) IRNode.distinct(1037,1059,1203,1229,1851,1959,2423,2531,2711,2733,2819,2841)
+        IRNode.inject(44,45) StoreFieldNode step.cases repDet evalDet option.distinct(1) Pair_inject
+        Value.inject(2) option.inject)
 next
   case (StaticStoreFieldNode nid f newval uv nxt m val h' h m')
   then have notseq: "\<not>(is_sequential_node (kind g nid))"
@@ -223,9 +224,9 @@ next
     by (simp add: StaticStoreFieldNode.hyps(1))
   from notseq notend notdivrem
   show ?case  
-    by (smt (verit) StoreFieldNode repDet evalDet StaticStoreFieldNode.hyps(1,2,3,4,5) Pair_inject
-        IRNode.distinct(1037,1203,1851,2423,2711,2733) IRNode.inject(44) option.distinct(1)
-        step.cases)
+    by (smt (verit) IRNode.distinct(1037,1059,1203,1229,1851,1959,2423,2531,2711,2733,2819,2841)
+        IRNode.inject(44,45) StoreFieldNode repDet evalDet StaticStoreFieldNode.hyps(1,2,3,4,5)
+        Pair_inject option.distinct(1) step.cases)
 next
   case (SignedDivNode nid x y zero sb nxt m v1 v2 v m' h)
   then have notseq: "\<not>(is_sequential_node (kind g nid))"
@@ -234,8 +235,8 @@ next
     by (simp add: SignedDivNode.hyps(1))
   from notseq notend
   show ?case  
-    by (smt (verit) SignedDivNode IRNode.distinct(1031,1197,1845,2417,2707,2711) IRNode.inject(41)
-        step.cases repDet evalDet Pair_inject)
+    by (smt (verit) IRNode.distinct(1031,1053,1197,1223,1845,1953,2417,2525,2707,2711,2815,2819)
+        IRNode.inject(42) SignedDivNode IRNode.inject(41) step.cases repDet evalDet Pair_inject)
 next
   case (SignedRemNode nid x y zero sb nxt m v1 v2 v m' h)
   then have notseq: "\<not>(is_sequential_node (kind g nid))"
@@ -244,8 +245,8 @@ next
     by (simp add: SignedRemNode.hyps(1))
   from notseq notend
   show ?case 
-    by (smt (verit) SignedRemNode IRNode.distinct(1033,1199,1847,2419,2707,2733) IRNode.inject(42)
-        step.cases repDet evalDet Pair_inject)
+    by (smt (verit) IRNode.distinct(1033,1055,1199,1225,1847,1955,2419,2527,2707,2733,2815,2841)
+        IRNode.inject(43) SignedRemNode IRNode.inject(42) step.cases repDet evalDet Pair_inject)
 qed
 
 lemma stepRefNode:
@@ -274,8 +275,7 @@ lemma step_in_ids:
   assumes "g, p \<turnstile> (nid, m, h) \<rightarrow> (nid', m', h')"
   shows "nid \<in> ids g"
   using assms apply (induct "(nid, m, h)" "(nid', m', h')" rule: step.induct) apply fastforce
-  apply (smt (z3) IRNode.distinct(1053,1219) IRNode.distinct_disc(2047) is_EndNode.simps(53)
-         is_AbstractEndNode.simps ids_some)+
-  by auto
+  by (metis IRNode.distinct(1075,1245,1975,2547,2835,2857,2895) IRNode.disc(1374,2895) ids_some
+      is_EndNode.simps(54) is_AbstractEndNode.simps)+
 
 end
